add implementation of emulator act and emulator trace. haven't yet implemented emulation

definitions.v
@@ -17,9 +17,13 @@ Definition all_tid := 0. (* XXX probably needs to change *)
 Inductive action : Type :=
 | ActInv (tid : tid) : action
 | ActResp (tid : tid) : action
-| Continue (tid: tid) : action.
+| Continue (tid: tid) : action
+| Emulate (tid: tid) : action
+| Commute (tid: tid) : action.
 Definition history : Type := list action.
 
+(* where the start of the commutative region of history begins *)
+Parameter commute_index : nat. 
 Definition thread_history_state : Type := tid -> nat.
 Definition thread_commute_state : Type := tid -> nat. (* 0 or 1 *)
 Definition refstate : Type := nat.
@@ -104,34 +108,106 @@ Hypothesis SIM_reordered_histories_correct : forall tr0 tr1 tr2 tr1' : trace,
     reordered (history_of_trace tr1) (history_of_trace tr1') ->
     List.In (history_of_trace (tr0 ++ tr1' ++ tr2)) spec.
 
+Definition thread_of_action (a: action) :=
+  match a with 
+  | ActInv t | ActResp t | Continue t
+  | Emulate t | Commute t => t
+  end.
+Definition action_eq (a1 a2: action) :=
+  match a1, a2 with
+  | Commute t, Commute t'
+  | Emulate t, Emulate t'
+  | ActInv t, ActInv t'
+  | ActResp t, ActResp t'
+  | Continue t, Continue t' => t =? t'
+  | _, _ => false
+  end.
 
-Definition emulator_trace (hbase hrun : history) : trace. Admitted.
+Definition inc_index (th : tid -> nat) (t: tid) :=
+  fun tid => if tid =? t then th tid + 1 else th tid.
+Definition set_index (tc : tid -> nat) (t : tid) :=
+  fun tid => if tid =? t then 1 else tc t.
+Definition enter_conflict_free_mode (hbase: history) (s: state) (t: tid) : state :=
+  match s with
+  | State rs th tc =>
+    let hd := nth (th t) hbase (Emulate t) in
+    let tc' := if action_eq hd (Commute t) then set_index tc t else tc in
+    let th' := if action_eq hd (Commute t) then inc_index th t else th in
+    State rs th' tc'
+  end.
+Definition should_switch_to_emulate (s : state) (hd a : action) (t : tid) : bool :=
+  match s with
+  | State rs th tc => 
+    eqb (action_eq hd a) false
+    && (eqb (action_eq a (Continue t)) false || eqb (action_eq hd (ActResp t)) false)
+    && eqb (action_eq hd (Emulate t)) false
+  end.
+Definition emulator_act
+           (hbase : history) (s : state) (a : action) : (state * action) :=
+  let t := thread_of_action a in
+  let s' := enter_conflict_free_mode hbase s t in
+  match s' with
+  | State rs th tc => 
+    let hd := nth (th t) hbase (Emulate t) in
+    (* do we need to switch to emulation mode? *)
+    let emulate_switch := should_switch_to_emulate s hd a t in
+    let th' := if emulate_switch then fun tid => (length hbase) + 1  (* always return Emulate *)
+               else th in
+    let rs' := if emulate_switch then rs (* TODO process H' or something*)
+              else rs in
+    (* actually emulate this step if we're emulating *)
+    if action_eq hd (Emulate t) then
+      let (rs'', r) := ref_impl (rs', a) in
+      (State rs'' th' tc, r)
+    (* if not, either in conflict-free mode or replaying *)
+    else let r := if action_eq hd a then Continue t
+                  else if action_eq a (Continue t) && action_eq hd (ActResp t)
+                       then hd
+                       else Continue t in (* XXX what if r is never set? need to prove that
+                                           * one of the conditions is always met? *)
+         let th'' := if tc t =? 1 then inc_index th' t (* conflict-free mode *)
+                    else fun tid => (th' tid) + 1 in (* replay *)
+         (State rs' th'' tc, r)
+  end.
+Function emulator_trace (hbase hrun : history) (s0 : state) (tr : trace) : trace :=
+  match hrun with
+  | [] => tr
+  | a :: rest => let (s', r) := emulator_act hbase s0 a in
+                 let t := thread_of_action a in
+                 emulator_trace hbase rest s' (Event t s0 s' a r :: tr)
+  end.
 
 (* if we have a correct trace whose corresponding history is SIM-comm,
  * then the emulator produces a conflict-free trace for that history *)
-Lemma emulator_impl_conflict_free : forall tr s0 s1,
+Lemma emulator_impl_conflict_free : forall t tr s0 s1,
     ref_impl_generated_trace tr s0 s1 ->
     sim_commutes (history_of_trace tr) ->
-    trace_conflict_free (emulator_trace (history_of_trace tr) (history_of_trace tr)).
+    trace_conflict_free (emulator_trace (Commute t :: (history_of_trace tr))
+                                        (history_of_trace tr)
+                                        s0 []).
 Proof.
 Admitted.
 
 (* if we have the emulator instantiated with a SIM-comm history,
  * and the emulator acts on some input sequence, then the emulator
  * produces a correct trace for the spec *)
-Lemma emulator_impl_correct : forall tr s0 s1 h,
+Lemma emulator_impl_correct : forall t tr s0 s1 h,
     ref_impl_generated_trace tr s0 s1 ->
     sim_commutes (history_of_trace tr) ->
-    List.In (history_of_trace (emulator_trace (history_of_trace tr) h)) spec.
+    List.In (history_of_trace (emulator_trace (Commute t :: history_of_trace tr)
+                                              h s0 []))
+            spec.
 Proof.
 Admitted.
 
-Theorem scalable_commutativity_rule : forall tr s0 s1 h,
+Theorem scalable_commutativity_rule : forall t tr s0 s1 h,
     ref_impl_generated_trace tr s0 s1 ->
     sim_commutes (history_of_trace tr) ->
-    trace_conflict_free (emulator_trace (history_of_trace tr) (history_of_trace tr))
-    /\
-    List.In (history_of_trace (emulator_trace (history_of_trace tr) h)) spec.
+    trace_conflict_free (emulator_trace (Commute t :: (history_of_trace tr))
+                                        (history_of_trace tr) s0 [])
+    /\ List.In
+         (history_of_trace (emulator_trace (Commute t :: history_of_trace tr) h s0 []))
+         spec.
 Proof.
   intros; split; [eapply emulator_impl_conflict_free | eapply emulator_impl_correct]; eauto.
 Qed.
